stuck at subs, coq doesn't know if subs will terminate

untyped_lambda.v
@@ -55,6 +55,7 @@ Notation "x :: l" := (cons x l)
 Notation "[ ]" := nil.
 Notation "[ x ; .. ; y ]" := (cons x .. (cons y nil) ..).
 
+
 (* I don't know how to import these notation ... *)
 
 Fixpoint remove_one(l : list var) (x : var) :=
@@ -86,15 +87,132 @@ Proof. reflexivity. Qed.
 Example FV_test2 : FV (App (Lambda (X 0) (Var (X 0))) (Var (X 0))) = [X 0].
 Proof. reflexivity. Qed.
 
-(* rename y as x in m, or m[y/x] *)
+(* rename y by x(whether free or not) in m , or m{y/x} *)
 
 Fixpoint renaming (m : term) (y x : var) : term :=
   match m with
   | Var xi => if var_eq xi x then Var y
               else Var xi
-  | Lambda xi m' =>  Var x
-  | App m1 m2 =>  Var x
-  end. (* TODO *)
+  | Lambda xi m' =>  if var_eq xi x
+                     then Lambda y (renaming m' y x)
+                     else Lambda xi (renaming m' y x)
+  | App m1 m2 =>  App (renaming m1 y x) (renaming m2 y x)
+  end. 
+
+
+(*   \x1.x0 x0   {x3/x0} *)
+Example renaming_test1 :
+  renaming (App (Lambda (X 1) (Var (X 0))) (Var (X 0))) (X 3) (X 0)  =
+           (App (Lambda (X 1) (Var (X 3))) (Var (X 3))).
+Proof. reflexivity. Qed.
+
+(* get all var in a term *)
+Fixpoint all_var (t : term) : list var :=
+  match t with
+  | Var x => [x]
+  | Lambda x t' => x :: all_var t'
+  | App t1 t2 => (all_var t1) ++ (all_var t2)
+  end.
+Example all_var_test1 :
+  all_var (App (Lambda (X 1) (Var (X 0))) (Var (X 4))) = [X 1; X 0; X 4].
+Proof. simpl. reflexivity. Qed.
+
+Fixpoint var_in_list (x : var) (l : list var) : bool :=
+  match l with
+  | [] => false
+  | h :: l' => if var_eq  x h then true else var_in_list x l'
+  end.
+Example var_in_list_test1:
+  var_in_list (X 3) [X 1; X 0; X 4] = false.
+Proof. reflexivity. Qed.
+Example var_in_list_test2:
+  var_in_list (X 4) [X 1; X 0; X 4] = true.
+Proof. reflexivity. Qed.
+
+
+
+(* \alpha-equivalence *)
+Axiom alpha_eq : forall (t:term) (x y:var),
+    not (In y (all_var t)) -> Lambda x t = Lambda y (renaming t y x).
+
+(* proof  \x1.x1 = \x0.x0 *)
+Example alpha_eq_test1:
+  Lambda (X 1) (Var (X 1)) = Lambda (X 0) (Var (X 0)).
+Proof.
+  replace (Lambda (X 0) (Var (X 0)))
+  with (Lambda (X 0) (renaming (Var (X 1)) (X 0) (X 1))).
+  apply alpha_eq.
+  simpl.
+  intros [h1 | h2].
+  - inversion h1. - exact h2.
+  - simpl. reflexivity.
+Qed.
+
+(* rules for alpha-equivalence:
+ refl:       M = M.
+ symm:       M = N -> N = M.
+ trans:      M = N -> N = P -> M = P
+ cong:       M = M' -> N = N' -> App M N = App M' N'
+ xi :        M = M' -> Lambda x M = Lambda x M'     
+ alpha       y \notin M ->  Lambda x M = Lambda y (M{y/x})
+*)
+Theorem refl : forall (M : term), M = M.
+Proof. intros. reflexivity. Qed.
+
+Theorem symm: forall (M N : term), M = N -> N = M.
+Proof. intros. symmetry. apply H. Qed.
+
+Theorem trans: forall (M N P : term), M = N -> N = P -> M = P.
+Proof. intros. rewrite H. apply H0. Qed.
+
+Theorem cong: forall (M N M' N' : term), M = M' ->  N = N' -> App M N = App M' N'.
+Proof. intros. rewrite H. rewrite H0. reflexivity. Qed.
+
+Theorem xi: forall(M M' : term) (x : var), M = M' -> Lambda x M = Lambda x M'.
+Proof. intros. rewrite H. reflexivity. Qed.
+
+Theorem alpha: forall (M : term) (x y: var),
+    ~(In y (all_var M)) -> Lambda x M = Lambda y (renaming M y x).
+Proof. apply alpha_eq. Qed.
+
+
+(** Substitution *)
+
+(* find var in a term having the biggest nat in it *)
+Definition max_var (M : term) : var :=
+  X (fold_right Nat.max 0 (map (fun v:var => match v with | X n => n end)
+                               (all_var M))).
+Theorem max_var_test1:  max_var (App (Lambda (X 1) (Var (X 5))) (Var (X 0))) = (X 5).
+Proof. reflexivity. Qed.
+
+Definition next_var (M : term) : var :=
+  X (S (fold_right Nat.max 0 (map (fun v:var => match v with | X n => n end)
+                               (all_var M)))).
+Theorem next_var_test1:  next_var (App (Lambda (X 1) (Var (X 5))) (Var (X 0))) = (X 6).
+Proof. reflexivity. Qed.
+
+
+(* M[N/x],  capture-avoiding, substitute free occurrences of x in M by N *)
+Fail Fixpoint subs (M N : term) (x : var) :=
+  match M with
+  | Var xi => if var_eq xi x then N else M
+  | App M1 M2 => App (subs M1 N x) (subs M2 N x)
+  | Lambda y M' =>  if var_eq y x
+                    then M
+                    else if negb (var_in_list y (FV N)) 
+                         then Lambda y (subs M' N x)
+                         else let y' := next_var (App M N) in
+                              Lambda y' (subs (renaming M' y' y) N x)
+  end.
+(* wooooooooooooooc                                       *)
+(* Error: Cannot guess decreasing argument of fix.        *)
+(* you can't write unterminate program in coq ??????!!!!! *)
+(* but renaming won't make M' bigger                      *)
+
+
+
+
+
 
 
 
